\documentclass{article}
\usepackage[utf8]{inputenc} % Required for inputting international characters
\usepackage[T1]{fontenc} % Output font encoding for international characters

\input{preamble}
\input{macros}

\graphicspath{{./images/}}

\title{\huge{9G and 9H}}
\author{\huge{Jack Maguire}}
\date{}

\begin{document}
\maketitle

\part*{9G}

\qs{3}{
\qsp{a}{
	\begin{multicols}{2}
		\noindent
		\[ \mandifferen{x}{t} = e^t \]
		\columnbreak
		\[ \mandifferen{y}{t} = e^t -e^{-t} \]
	\end{multicols}
	\begin{align*}
		\differen &= \frac{e^t -e^{-t}}{e^t} \\
		&= \frac{e^t}{e^t} - \frac{e^{-t}}{e^t} \\
		&= 1 - e^{-2t} \\ \\
		t &= 0 \\
		\differen &= 1 - e^0 \\
		&= 0 \\
	\end{align*}
	\begin{multicols}{2}
		\noindent
		\[ x = e^0 = 1 \]
		\columnbreak
		\[ y = e^0 + e^0 = 2 \]
	\end{multicols}
	\begin{align*}
		y - y_1 &= m\left( x - x_1 \right) \\
		y - 2 &= 0 * (\ldots) \\
		y &= 2 \\
	\end{align*}
}
\qsp{b}{
	\begin{multicols}{2}
		\noindent
		\[ \mandifferen{x}{t} = 2 \sin 2t \]
		\columnbreak
		\[ \mandifferen{y}{t} = 2 \cos 2t  \]
	\end{multicols}
	\begin{align*}
		\differen &= \frac{2 \cos 2t}{2 \sin 2t} \\
		&= \cot 2t \\ \\
		t &= \frac{\pi}{6} \\
		\differen &= \cot \frac{\pi}{3} \\
		&= \frac{\sqrt{3}}{3}
	\end{align*}
	\begin{multicols}{2}
		\noindent
		\[ x = 1 - \cos \frac{\pi}{3} = \frac{1}{2} \]
		\columnbreak
		\[ y = \sin \frac{\pi}{3} = \frac{\sqrt{3}}{2} \]
	\end{multicols}
	\begin{align*}
		y - y_1 &= m \left( x - x_1 \right) \\
		y - \frac{\sqrt{3}}{2} &= \frac{\sqrt{3}}{3} \left( x - \frac{1}{2} \right) \\
		y - \frac{\sqrt{3}}{2} &= \frac{\sqrt{3}}{3} x - \frac{\sqrt{3}}{6} \\
		y &= \frac{\sqrt{3}}{3} x + \frac{\sqrt{3}}{3}
	\end{align*}
}
}

\qs{4}{
\begin{multicols}{2}
	\noindent
	\begin{align*}
		x &= \frac{t}{1-t} \\
		\mandifferen{x}{t} &= \frac{vu^\prime - v^\prime u}{v^2} \\
		&= \frac{1-t + t}{1 - 2t + t^2} \\
		&= \frac{1}{t^2 - 2t + 1}
	\end{align*}
	\columnbreak
	\begin{align*}
		y &= \frac{t^2}{1-t} \\
		\mandifferen{y}{t} &= \frac{vu^\prime - v^\prime u}{v^2} \\
		&= \frac{2t\left( 1-t \right) + t^2}{1 - 2t + t^2} \\
		&= \frac{2t - t^2}{t^2 - 2t + 1}
	\end{align*}
\end{multicols}
\begin{align*}
	\differen &= \frac{2t - t^2}{1 - 2t + t^2} \div \frac{1}{t^2 - 2t + 1} \\
	&= \frac{\left( 2t - t^2 \right) \left( t^2 - 2t + 1 \right)}{t^2 - 2t + 1} \\
	&= 2t - t^2 \\
	0 &= 2t - t^2 \\
	t &= 0, 2
\end{align*}
\begin{multicols}{2}
	\noindent
	\begin{align*}
		t &= 0 \\
		x &= \frac{t}{1-t} \\
		&= 0 \\
		y &= \frac{t^2}{1-t} \\
		&= 0
	\end{align*}
	\columnbreak
	\begin{align*}
		t &= 2 \\
		x &= \frac{t}{1-t} \\
		&= -2 \\
		y &= \frac{t^2}{1-t} \\
		&= -4
	\end{align*}
\end{multicols}
\[ = (0, 0), (-2, -4) \]
}

\pagebreak
\part*{9H}

\qs{4}{
\begin{align*}
	0 &= 2x + 6xy \differen + 3y^2 - 3y^2 \differen \\
	-2x - 3y^2 &= 6xy \differen - 3y^2 \differen \\
	\differen &= \frac{-2x - 3y^2}{6xy - 3y^2} \\
	&= -\frac{3y^2 + 2x}{3y^2 - 6xy} \\ \\
	&= -\frac{3*1^2 + 2*2}{3*1^2 - 6*2*1} \\
	&= -\frac{7}{9}
\end{align*}
}

\qs{5}{
\begin{align*}
	2x + \differen &= 3(x+y)^2\left( 1 + \differen \right) \\
	2x + \differen &= 3(x+y)^2 + 3\differen(x+y)^2 \\
	3(x+y)^2 - 2x &= \differen - 3\differen(x+y)^2 \\
	\differen &= \frac{3(x+y)^2 - 2x}{1 - 3(x+y)^2} \\ \\
	&= \frac{3(1+0)^2 - 2*1}{1 - 3(1+0)^2} \\
	&= -\frac{1}{2} \\
\end{align*}
}
	
\end{document}